# Math 375

#### Geonho Roh

1)
$$
\text{Show that if }f(x)=|x|\text{ then for any number }m
\\ \lim_{h\rightarrow0}(f(h+0)-f(0)-mh)=0 
\\ \text{ but}
\\ \lim_{h\rightarrow0}\frac{1}{h}(f(h+0)-f(0)-mh)=0
\\ \text{never holds, what does this say about }f
$$

$$
\lim_{h\rightarrow0}(f(h+0)-f(0)-mh)=0 \text{ since every parts convergence}
\\ \lim_{h\rightarrow0}f(h+0)-\lim_{h\rightarrow0}f(0)-\lim_{h\rightarrow0}mh
\\ =0+0+0=0
\\
\\
\\ \lim_{h\rightarrow0}\frac{1}{h}(f(h+0)-f(0)-mh)=0
\\ \lim_{h\rightarrow0^+}\frac{1}{h}(f(h+0)-f(0)-mh)\neq\lim_{h\rightarrow0^-}\frac{1}{h}(f(h+0)-f(0)-mh)
\\ \lim_{h\rightarrow0^+}\frac{1}{h}(f(h+0)-f(0)-mh)=1-m
\\ \lim_{h\rightarrow0^-}\frac{1}{h}(f(h+0)-f(0)-mh)=-1-m
\\ \lim_{h\rightarrow0}\frac{1}{h}(f(h+0)-f(0)-mh) \text{ cannot be defined}
\\ \text{therefore it never holds}
\\
\\ \text{it means }f \text{ is not differentiable at 0}
$$

2)
$$
\text{Find the Jacobian matrices of the following maps. Show your work.}
\\
\\\text{1) }f(x,y)=e^{x^2+y^3}
\\ \text{2) }f(x,y)=(xy,sin(xy))
$$

$$
\text{1) }f(x,y)=e^{x^2+y^3}
\\
\\ Df(x,y)=\begin{bmatrix}\partial f/\partial x,\partial f/\partial y\end{bmatrix}
\\= \begin{bmatrix}\partial f/\partial x,\partial f/\partial y\end{bmatrix}
\\=[2xe^{x^2+y^3},3ye^{x^2+y^3}]
\\
\\ \text{2) }f(x,y)=(xy,sin(xy))
\\
\\ Df(x,y)=\begin{bmatrix}\partial f_1/\partial x&&\partial f_1/\partial y\\\partial f_2/\partial x&&\partial f_2/\partial y \end{bmatrix}
\\=\begin{bmatrix}y&&x\\ycos(xy)&&xcos(xy) \end{bmatrix}
$$

3)
$$
\text{Consider the following function }f: \R^2 \rightarrow \R
\\ \text{ given by }
\\
\\ f(x,y)=\frac{x^4+y^4}{x^2+y^2} \text{ if }(x,y)\neq 0
\\   = (0,0 )\text{ if }(x,y)= 0
\\ \text{show that it is differentiable at }(0,0)
$$

$$
\text{for }f(x,y)\text{ to be differentiable }
\\ \text{ it has to satisfy }
\\ \lim_{(x,y)\rightarrow(0,0)}\frac{f(x,y)-f(0,0)-T_{(0,0)}|(x,y)-(0,0)|}{||(x,y)-(0,0)||}=0
\\	\lim_{(x,y)\rightarrow(0,0)}\frac{\frac{x^4+y^4}{x^2+y^2}-0-f_x(0,0)x-f_y(0,0)y}{\sqrt{x^2+y^2} }
\\
\\ f_x(0,0) = \lim_{h\rightarrow0}\frac{f(h,0)-f(0,0)}{h}=h=0
\\ f_y(0,0) = \lim_{h\rightarrow0}\frac{f(0,h)-f(0,0)}{h}=h=0
\\
\\ \lim_{(x,y)\rightarrow(0,0)}\frac{\frac{x^4+y^4}{x^2+y^2}-0-f_x(0,0)x-f_y(0,0)y}{\sqrt{x^2+y^2} }
\\ = \lim_{(x,y)\rightarrow(0,0)}\frac{\frac{x^4+y^4}{x^2+y^2}}{\sqrt{x^2+y^2} }
\\ = \lim_{(x,y)\rightarrow(0,0)}{\frac{x^4+y^4}{(x^2+y^2)\sqrt{x^2+y^2} }}
\\
\\ \text{using squeeze theorem }
$$


$$
0\leq\lim_{(x,y)\rightarrow(0,0)}{\frac{x^4+y^4}{(x^2+y^2)\sqrt{x^2+y^2} }}\leq\lim_{(x,y)\rightarrow(0,0)}{\frac{(x^2+y^2)^2}{(x^2+y^2)\sqrt{x^2+y^2} }}
\\0\leq\lim_{(x,y)\rightarrow(0,0)}{\frac{x^4+y^4}{(x^2+y^2)\sqrt{x^2+y^2} }}\leq\lim_{(x,y)\rightarrow(0,0)}\sqrt{x^2+y^2}
\\0\leq\lim_{(x,y)\rightarrow(0,0)}{\frac{x^4+y^4}{(x^2+y^2)\sqrt{x^2+y^2} }}\leq0
\\ \lim_{(x,y)\rightarrow(0,0)}{\frac{x^4+y^4}{(x^2+y^2)}}=0
\\
\\ \text{Therefore }f(x,y)\text{ is differentiable at }(0,0)
$$
4)
$$
\text{Consider the following function }f: \R^2 \rightarrow \R
\\ \text{ given by }
\\
\\ f(x,y)=\frac{x^3}{x^2+y^2} \text{ if }(x,y)\neq 0
\\   = (0,0 )\text{ if }(x,y)= 0
\\ \text{show that it has jacobian but not differentiable at }(0,0)
$$

$$
\text{Jacobian	}
\\ [\partial f/\partial x,\partial f/\partial y]
\\ \text{at }(0,0)
\\ [\lim_{h\rightarrow0}\frac{f(h,0)-f(0,0)}{h},\lim_{h\rightarrow0}\frac{f(0,h)-f(0,0)}{h}]
\\ = [1,0]
\\ \text{so it exist}
\\
\\ \text{Differentiability }
\\ \text{ it has to satisfy }
\\ \lim_{(x,y)\rightarrow(0,0)}\frac{f(x,y)-f(0,0)-T_{(0,0)}|(x,y)-(0,0)|}{||(x,y)-(0,0)||}=0
\\	\lim_{(x,y)\rightarrow(0,0)}\frac{\frac{x^3}{x^2+y^2}-0-f_x(0,0)x-f_y(0,0)y}{\sqrt{x^2+y^2} }
\\
\\ f_x(0,0) = 1
\\ f_y(0,0) = 0
\\
\\\lim_{(x,y)\rightarrow(0,0)}\frac{\frac{x^3}{x^2+y^2}-x}{\sqrt{x^2+y^2} }
\\ \lim_{(x,y)\rightarrow(0,0)}\frac{\frac{-xy^2}{x^2+y^2}}{\sqrt{x^2+y^2} }
\\ \lim_{(x,y)\rightarrow(0,0)}{\frac{-xy^2}{(x^2+y^2)\sqrt{x^2+y^2}}}
\\ \text{along }y=mx
\\ \lim_{x\rightarrow0}{\frac{-xm^2x^2}{(x^2+m^2x^2)\sqrt{x^2+m^2x^2}}}
\\ \lim_{x\rightarrow0}{\frac{-x^3m^2}{x^2(1+m^2)x\sqrt{1+m^2}}}
\\ \lim_{x\rightarrow0}{\frac{-m^2}{(1+m^2)\sqrt{1+m^2}}}
\\
\\ \lim_{x\rightarrow0}{\frac{-m^2}{(1+m^2)\sqrt{1+m^2}}} \text{ is not always }0
\\
\\ \text{therefore it is not differentiable}
$$

5) Apostol Section 8.9 Problem 13 

$$
\text{compute all first-order partial derivatives}
\\
\\  f(x, y) = \tan(x^2/y), y\neq0
\\ \partial f/\partial x=\frac{2x}{y}\sec^2(x^2/y)
\\ \partial f/\partial y=\frac{-x^2}{y^2}\sec^2(x^2/y)
$$

6. Apostol Section 8.14 Problem 2

$$
\text{Evaluate the directional derivatives of the following scalar fields for the points and directions
given :}
$$

$$
\text{a) }f(x,y,z)=x^2+2y^2+3z^2 \text{ at }(1,1,0) \text{ in the direction of }i-j+2k
\\
\\ \lim_{h\rightarrow0}\frac{f(1,1,0+h(1,-1,2))-f(1,1,0)}{h}
\\ \lim_{h\rightarrow0}\frac{f(1+h,1-h,2h)-f(1,1,0)}{h}
\\ \lim_{h\rightarrow0}\frac{f(1+h,1-h,2h)-f(1,1,0)}{h}
\\ =\lim_{h\rightarrow0}\frac{15h^2-2h}{h}
\\ =-2
\\ 
\\ \text{divide by norm}
\\ \frac{-2}{\sqrt6}
$$

$$
\text{b) }f(x,y,z)=(x/y)^z \text{ at (1,1,1) in direction of }(2,1,-1)
\\
\\ D_{(2,1,-1)}f_{(1,1,1) }=f_x(1,1,1) 2+f_y(1,1,1)1+f_z(1,1,1)(-1)
\\ f_x=zy^{-z}x^{z-1},f_y=-zx^zy^{-z-1},f_z=(x/y)^z\ln(x/y)
\\ f_x(1,1,1) 2+f_y(1,1,1)1+f_z(1,1,1)(-1)=1
\\ \text{divide by norm }\frac{1}{\sqrt 6}
\\
\\ \text{Since the quality of pdf is too bad i am not sure }f(x,y,z)=(x/y)^z \text{ or }f(x,y,z)=(x/y)^2
\\
\\ \text{If }f(x,y,z)=(x/y)^2
\\
\\ D_{(2,1,-1)}f_{(1,1,1) }=f_x(1,1,1) 2+f_y(1,1,1)1+f_z(1,1,1)(-1)
\\ f_x=2y^{-2}x,f_y=-2x^2y^{-3},f_z=0
\\ f_x(1,1,1) 2+f_y(1,1,1)1+f_z(1,1,1)(-1)=2
\\ \text{divide by norm }\frac{2}{\sqrt 6}
$$

7.
$$
\text{Let }f:\R^3\rightarrow \R^2 \text{ satisfy the condition }f(\vec 0)=(1,2)
\\ Df(\vec0)=\begin{bmatrix}1&2&3\\0&0&1 \end{bmatrix}
\\ \text{let }g:\R^2\rightarrow \R^2 \text{ be }g(x,y)=(x+2y+1,3xy)
\\ \text{find }D(g \circ f)(\vec 0)
$$

$$
\text{Using chainrule }
\\ D(g\circ f)(\vec 0) = D(g)(f(\vec 0))D(f)(\vec 0) 
\\

\\ D(f)(\vec 0)=\begin{bmatrix}1&2&3\\0&0&1 \end{bmatrix}
\\D(g)(f(\vec 0))
\\ =\begin{bmatrix}1&2\\3y&3x \end{bmatrix}_{(1,2)}
\\=\begin{bmatrix}1&2\\6&3 \end{bmatrix}
\\
\\ \begin{bmatrix}1&2\\6&3 \end{bmatrix}\begin{bmatrix}1&2&3\\0&0&1 \end{bmatrix}
\\=\begin{bmatrix}1&2&5\\6&12&21 \end{bmatrix}
\\
\\  D(g\circ f)(\vec 0) =\begin{bmatrix}1&2&5\\6&12&21 \end{bmatrix}
$$

8.
$$
\text{Let }f:\R^3 \rightarrow \R^2 \text{ Let }g:\R^2\rightarrow \R \text{ be differentiable }
\\ F:\R^2\rightarrow \R\text{ be defined by} 
\\ F:(x,y)=f(x,y,g(x,y))
\\
\\ \text{a) find DF in term of partials of f and g}
\\ \text{b) if F(x,y)=0 for all (x,y), find }D_1g \text{ and }D_2g \text{ in terms of the partials of }f
$$

$$
\\ D_1f(x,y,g(x,y)),D_3f(x,y,g(x,y)),D_1g(x,y),D_2f(x,y,g(x,y)),dot D_2g(x,y)
\\ \text{briefly write }
\\  D_1f,D_2f,D_3f,D_1g,D_2g
\\
\\
\text{a) find DF in term of partials of f and g}
\\
\\F(x,y)=f(x,y,g(x,y)) \text{ so }F=f\circ h
\\
\\ DF=(D_1F,D_2F)
\\ =(D_1f+D_3f\cdot D_1g,D_2f+D_3f\cdot D_2g) 
\\ 
$$

---

$$
\text{b) if F(x,y)=0 for all (x,y), find }D_1g \text{ and }D_2g \text{ in terms of the partials of }f
\\
\\ \text{if F(x,y)=0 for all (x,y) that means }DF=0
\\(D_1f+D_3f\cdot D_1g,D_2f+D_3f\cdot D_2g)=(0,0)
\\ D_1f+D_3f\cdot D_1g=0
\\ D_1g=-D_1f/D_3f
\\
\\D_2f+D_3f\cdot D_2g=0
\\D_2g=-D_2f/D_3f
$$





