# Math 375

### Geonho Roh	

(1) 2.12 Pr 10 

$$
\text{Let }V \text{ and } W \text{ be linear spaces, each with dimension 2 and each with basis }(e_1 , e_2). \\ \text{Let }T: V\rightarrow W \text{ be a linear transformation such that }T(e_1 + e_2) = 3e_1 + 9e_2,
\\ T(3e_1 + 2e_2) = 7e_1 + 23e_2.
$$

$$
\text{a) Compute }T(e_2-e_1) \text{  and determine the nullity and rank of }T
\\
\\T(e_1 + e_2) = 3e_1 + 9e_2
\\ T(3e_1 + 2e_2) = 7e_1 + 23e_2
\\
\\T(e_1)+T(e_2)= 3e_1 + 9e_2
\\3T(e_1)+2T(e_2)= 7e_1 + 23e_2
\\ T(e_1)= e_1+5e_2
\\ T(e_2)=2e_1+4e_2
\\\\
\\T(e_2-e_1)=T(e_2)-T(e_1)=2e_1+4e_2-(e_1+5e_2)
\\=e_1-e_2
\\
\\ T(e_1)=e_1+5e_2=(1)e_1+(5)e_2=\left[ \begin{matrix} 1 \\5 \end{matrix} \right]
\\ T(e_2)=2e_1+4e_2=(2)e_1+(4)e_2=\left[ \begin{matrix} 2 \\4\end{matrix} \right]
\\
\\ [T]=\left[ \begin{matrix} 1&2 \\5&4 \end{matrix} \right]
\\
\\ \text{Therefore }T(v) ,v=\left[ \begin{matrix}x_1\\x_2\end{matrix} \right] v \in V 
\\T(v)=\left[ \begin{matrix} 1&2 \\5&4 \end{matrix} \right]\left[ \begin{matrix}x_1\\x_2\end{matrix} \right] =\left[ \begin{matrix}x_1+2x_2\\5x_1+4x_2\end{matrix} \right]
\\ 
\\ \text{When }x_1=x_2=0
\\\left[ \begin{matrix}x_1+2x_2\\5x_1+4x_2\end{matrix} \right]=\left[ \begin{matrix}0\\0\end{matrix} \right]
\\\text{So Nullity is }0
\\
\\ \text{The range is spanned by }\left[ \begin{matrix} 1 \\5 \end{matrix} \right]\left[ \begin{matrix} 2 \\4\end{matrix} \right] 
\\ \text{Therefore Rank is }2
$$



-------------


$$
\text{b) Determine the matrix of }T \text{ relative to given matrix}
\\
\\ \text{In a) we get the matrix of }T
\\ [T]=\left[ \begin{matrix} 1&2 \\5&4 \end{matrix} \right]
$$

--------

$$
\text{c) Use the basis } (e_1 , e_2) \text{ for V and find a new basis of the form }(e_1 + ae_2, 2e_1, + be_2)
\\ \text{ for W,
relative to which the matrix of T will be in diagonal form }
\\
\\ \text{Let }e_1 + ae_2=e_1 + 5e_2 \text{ and }2e_1, + be_2=2e_1, + 4e_2
\\ T(e_1)=(a_1)e_1 + 5e_2 +(a_2)2e_1, + 4e_2
\\ T(e_2)=(b_1)e_1 + 5e_2 +(b_2)2e_1, + 4e_2
\\ \text{To be diagonal }a_2=b_1=0
\\
\\ T(e_1)=(a_1)e_1 + 5e_2
\\ T(e_2)=(b_2)2e_1, + 4e_2
\\
\\ \text{Since }
\\ T(e_1)=e_1+5e_2=(1)e_1+(5)e_2=\left[ \begin{matrix} 1 \\5 \end{matrix} \right]
\\ T(e_2)=2e_1+4e_2=(2)e_1+(4)e_2=\left[ \begin{matrix} 2 \\4\end{matrix} \right]
\\ a_1=b_2=1
\\ [T]=\left[ \begin{matrix} 1&0 \\0&1\end{matrix} \right]
\\ 
\\ \text{Therefore the basis of W is }(e_1 + 5e_2,2e_1, + 4e_2)
$$

(2) 2.16 Pr 6
$$
\text{Let }A=\left[ \begin{matrix} 1&1 \\0&1\end{matrix} \right] \text{ Verify that }A^2=\left[ \begin{matrix} 1&2 \\0&1\end{matrix} \right] \text{ and compute }A^n
\\
\\ A^2=\left[ \begin{matrix} 1&1 \\0&1\end{matrix} \right] \left[ \begin{matrix} 1&1 \\0&1\end{matrix} \right] 
\\=\left[ \begin{matrix} 1+0&1+1 \\0+0&0+1\end{matrix} \right] =\left[ \begin{matrix} 1&2 \\0&1\end{matrix} \right] 
\\
\\ \text{Going to prove }A^n=\left[ \begin{matrix} 1&n \\0&1\end{matrix} \right] \text{ for all integers using induction}
\\ \text{basic step is already showed}
\\
\\ \text{Assume that it is true when n then prove for n+1}
\\ A^n=\left[ \begin{matrix} 1&n \\0&1\end{matrix} \right] 
\\ A^{n+1}=\left[ \begin{matrix} 1&n \\0&1\end{matrix} \right] \left[ \begin{matrix} 1&1 \\0&1\end{matrix} \right]
\\ = \left[ \begin{matrix} 1+0&1+n \\0+0&0+1\end{matrix} \right]=\left[ \begin{matrix} 1&1+n \\0&1\end{matrix} \right]
\\
\\ \text{Therefore }A^{n+1}=\left[ \begin{matrix} 1&1+n \\0&1\end{matrix} \right] \text{ So it is true when }n+1
\\
\\ \text{By induction }A^n=\left[ \begin{matrix} 1&n \\0&1\end{matrix} \right]
$$
(3) 2.16 Pr 9 
$$
\text{Let }A=\left[ \begin{matrix} 1&0 \\-1&1\end{matrix} \right] \text{ Prove that }A^2=2A-Z \text{ and compute }A^{100}
\\
\\ A^2=\left[ \begin{matrix} 1&0 \\-1&1\end{matrix} \right]\left[ \begin{matrix} 1&0 \\-1&1\end{matrix} \right]
\\=\left[ \begin{matrix} 1+0&0+0 \\-1-1&0+1\end{matrix} \right]=\left[ \begin{matrix} 1&0 \\-2&1\end{matrix} \right]
\\
\\2A-Z=2\left[ \begin{matrix} 1&0 \\-1&1\end{matrix} \right]-\left[ \begin{matrix} 1&0 \\0&1\end{matrix} \right]  
\\=\left[ \begin{matrix} 2&0 \\-2&2\end{matrix} \right]-\left[ \begin{matrix} 1&0 \\0&1\end{matrix} \right]
\\=\left[ \begin{matrix} 1&0 \\-2&1\end{matrix} \right]
\\  \text{Therefore }A^2=2A-Z
\\
$$

$$
\\ \text{Going to prove }A^n=\left[ \begin{matrix} 1&0 \\-n&1\end{matrix} \right] \text{ for all integers using induction}
\\ \text{basic step is already showed}
\\
\\ \text{Assume that it is true when n then prove for n+1}
\\ A^n=\left[ \begin{matrix} 1&0 \\-n&1\end{matrix} \right] 
\\ A^{n+1}=\left[ \begin{matrix} 1&0 \\-n&1\end{matrix} \right]  \left[ \begin{matrix} 1&0 \\-1&1\end{matrix} \right]
\\ = \left[ \begin{matrix} 1+0&0+0 \\-n-1&0+1\end{matrix} \right]=\left[ \begin{matrix} 1&0 \\-n-1&1\end{matrix} \right]
\\
\\ \text{Therefore }A^{n+1}=\left[ \begin{matrix} 1&0 \\-n-1&1\end{matrix} \right] \text{ So it is true when }n+1
\\
\\ \text{By induction }A^n=\left[ \begin{matrix} 1&0 \\-n&1\end{matrix} \right]
\\
\\ \text{Therefore }A^{100}=\left[ \begin{matrix} 1&0 \\-100&1\end{matrix} \right]
\\
$$

(4) 2.16 Pr 11 
$$
\text{a) Prove that a }2\times2 \text{ matrix }A \text{ commutes with every }2\times2 \text{ matrix if and only if }
\\A \text{ commutes with each of the four matrices}
\\ \left[ \begin{matrix} 1&0 \\0&0\end{matrix} \right],\left[ \begin{matrix} 0&0 \\0&1\end{matrix} \right]
,\left[ \begin{matrix} 0&1 \\0&0\end{matrix} \right],\left[ \begin{matrix} 0&0 \\1&0\end{matrix} \right]
\\
\\ \text{first prove }\rightarrow \text{ direction}
\\ \text{let }\left[ \begin{matrix} a&b \\c&d\end{matrix} \right]\text{ arbitary }2\times2 \text{ matrix}
\\ \text{then }A\left[ \begin{matrix} a&b \\c&d\end{matrix} \right]=\left[ \begin{matrix} a&b \\c&d\end{matrix} \right]A
\\
\\\left[ \begin{matrix} a&b \\c&d\end{matrix} \right]=a\left[ \begin{matrix} 1&0 \\0&0\end{matrix} \right]+b\left[ \begin{matrix} 0&1 \\0&0\end{matrix} \right]+c\left[ \begin{matrix} 0&0 \\1&0\end{matrix} \right]+d\left[ \begin{matrix} 0&0 \\0&1\end{matrix} \right]
\\
\\A(a\left[ \begin{matrix} 1&0 \\0&0\end{matrix} \right]+b\left[ \begin{matrix} 0&1 \\0&0\end{matrix} \right]+c\left[ \begin{matrix} 0&0 \\1&0\end{matrix} \right]+d\left[ \begin{matrix} 0&0 \\0&1\end{matrix} \right])=(a\left[ \begin{matrix} 1&0 \\0&0\end{matrix} \right]+b\left[ \begin{matrix} 0&1 \\0&0\end{matrix} \right]+c\left[ \begin{matrix} 0&0 \\1&0\end{matrix} \right]+d\left[ \begin{matrix} 0&0 \\0&1\end{matrix} \right])A
\\
\\(aA\left[ \begin{matrix} 1&0 \\0&0\end{matrix} \right]+bA\left[ \begin{matrix} 0&1 \\0&0\end{matrix} \right]+cA\left[ \begin{matrix} 0&0 \\1&0\end{matrix} \right]+dA\left[ \begin{matrix} 0&0 \\0&1\end{matrix} \right])=(a\left[ \begin{matrix} 1&0 \\0&0\end{matrix} \right]A+b\left[ \begin{matrix} 0&1 \\0&0\end{matrix} \right]A+c\left[ \begin{matrix} 0&0 \\1&0\end{matrix} \right]A+d\left[ \begin{matrix} 0&0 \\0&1\end{matrix} \right]A)
\\ \text{Therefore A commutes with the four matrices}
\\
$$

$$
\text{Prove }\leftarrow \text{ direction }
\\ \text{A commutes with the four matrices } 
\\
\\
\\ \text{As we showed above}
\\A\left[ \begin{matrix} a&b \\c&d\end{matrix} \right]=A(a\left[ \begin{matrix} 1&0 \\0&0\end{matrix} \right]+b\left[ \begin{matrix} 0&1 \\0&0\end{matrix} \right]+c\left[ \begin{matrix} 0&0 \\1&0\end{matrix} \right]+d\left[ \begin{matrix} 0&0 \\0&1\end{matrix} \right])
\\
\\ \text{Since }A \text{ commutes with the four matrices }
\\A(a\left[ \begin{matrix} 1&0 \\0&0\end{matrix} \right]+b\left[ \begin{matrix} 0&1 \\0&0\end{matrix} \right]+c\left[ \begin{matrix} 0&0 \\1&0\end{matrix} \right]+d\left[ \begin{matrix} 0&0 \\0&1\end{matrix} \right])
\\=(aA\left[ \begin{matrix} 1&0 \\0&0\end{matrix} \right]+bA\left[ \begin{matrix} 0&1 \\0&0\end{matrix} \right]+cA\left[ \begin{matrix} 0&0 \\1&0\end{matrix} \right]+dA\left[ \begin{matrix} 0&0 \\0&1\end{matrix} \right])
\\=(a\left[ \begin{matrix} 1&0 \\0&0\end{matrix} \right]A+b\left[ \begin{matrix} 0&1 \\0&0\end{matrix} \right]A+c\left[ \begin{matrix} 0&0 \\1&0\end{matrix} \right]A+d\left[ \begin{matrix} 0&0 \\0&1\end{matrix} \right]A)
\\=(a\left[ \begin{matrix} 1&0 \\0&0\end{matrix} \right]+b\left[ \begin{matrix} 0&1 \\0&0\end{matrix} \right]+c\left[ \begin{matrix} 0&0 \\1&0\end{matrix} \right]+d\left[ \begin{matrix} 0&0 \\0&1\end{matrix} \right])A
\\=\left[ \begin{matrix} a&b \\c&d\end{matrix} \right]A
$$

(5) 2.20 Pr 2 
$$
\text{Do Gaussian Jordan Elimination and find solution if exist}
\\
\\3x+2y+z=1
\\5x+3y+3z=2
\\x+y-z=1
\\
\\\left[ \begin{matrix} 3&2&1 \\5&3&3\\1&1&-1\end{matrix} \right]\left[ \begin{matrix} 1 \\ 2 \\1\end{matrix} \right]
\\ \left[ \begin{matrix}1&1&-1\\ 3&2&1 \\5&3&3\end{matrix} \right]\left[ \begin{matrix} 1 \\ 2 \\1\end{matrix} \right]
\\ \left[ \begin{matrix}1&1&-1\\ 0&-2&8 \\0&-1&4\end{matrix} \right]\left[ \begin{matrix} 1 \\ -3 \\-2\end{matrix} \right]
\\ \left[ \begin{matrix}1&1&-1\\ 0&1&-4 \\0&-1&4\end{matrix} \right]\left[ \begin{matrix} 1 \\ \frac{3}{2} \\-2\end{matrix} \right]
\\ \left[ \begin{matrix}1&1&-1\\ 0&1&-4 \\0&0&0\end{matrix} \right]\left[ \begin{matrix} 1 \\ \frac{3}{2} \\\frac{-1}{2}\end{matrix} \right]
\\
\\ \text{In the process we found that the last equation }0x+0y+0z=\frac{-1}{2}
\\ \text{Therefore there is no solution}
$$
(6) 2.20 Pr 6 
$$
x+y-3z+u=5
\\2x-y+ z-2u=2
\\7x+y-7z+3u=3
\\
\\\\ \left[ \begin{matrix}1&1&-3&1\\ 2&-1&1&-2 \\7&1&-7&3\end{matrix} \right]\left[ \begin{matrix} 5\\ 2 \\3\end{matrix} \right]
\\\\ \left[ \begin{matrix}1&1&-3&1\\ 0&-3&7&-4 \\0&-6&14&-4\end{matrix} \right]\left[ \begin{matrix} 5\\ -8 \\-32\end{matrix} \right]
\\\\ \left[ \begin{matrix}1&1&-3&1\\ 0&1&\frac{-7}{3}&\frac{4}{3} \\0&-6&14&-4\end{matrix} \right]\left[ \begin{matrix} 5\\ \frac{8}{3} \\-32\end{matrix} \right]
\\\\ \left[ \begin{matrix}1&1&-3&1\\ 0&1&\frac{-7}{3}&\frac{4}{3} \\0&0&0&1\end{matrix} \right]\left[ \begin{matrix} 5\\ \frac{8}{3} \\-4\end{matrix} \right]
\\\\ \left[ \begin{matrix}1&0&\frac{-2}{3}&0\\ 0&1&\frac{-7}{3}&0\\0&0&0&1\end{matrix} \right]\left[ \begin{matrix} 1\\8 \\-4\end{matrix} \right]
\\
$$

$$
\\ x-\frac{2}{3}z=1
\\y-\frac{7}{3}z=8
\\u=-4
\\
\\ \text{let }z=a
\\ x=1+\frac{2}{3}a
\\ y =8+\frac{7}{3}a
\\u=-4
\\
\\ (x,y,z,u)=(1+\frac{2}{3}a,8+\frac{7}{3}a,a,-4)
\\ =a(\frac{2}{3},\frac{7}{3},1,0)+(1,8,0,-4) \
$$

(7) 2.20 Pr 10 
$$
\text{Determine all solutions of the system}
$$

$$
5x+2y-6z+2u=-1
\\x-y+z-u=-2
\\
\\ \left[ \begin{matrix}5&2&-6&2\\ 1&-1&1&-1 \end{matrix} \right]\left[ \begin{matrix} -1 \\-2\end{matrix} \right]
\\\left[ \begin{matrix}1&-1&1&-1\\ 5&2&-6&2 \end{matrix} \right]\left[ \begin{matrix} -2 \\-1\end{matrix} \right]
\\\left[ \begin{matrix}1&-1&1&-1\\ 0&7&-11&7 \end{matrix} \right]\left[ \begin{matrix} -2 \\9\end{matrix} \right]
\\\left[ \begin{matrix}1&-1&1&-1\\ 0&1&-\frac{11}{7}&1 \end{matrix} \right]\left[ \begin{matrix} -2 \\\frac{9}{7}\end{matrix} \right]
\\\left[ \begin{matrix}1&0&-\frac{4}{7}&0\\ 0&1&-\frac{11}{7}&1\end{matrix} \right]\left[ \begin{matrix} -\frac{5}{7} \\\frac{9}{7}\end{matrix} \right]
\\
\\ 7x-4z=-5
\\ 7y-11z+u=9
\\
\\ \text{let }z=a, u=b
\\ x=(-5+4a)/7 , y=(9+11a-b)/7
\\
\\ (x,y,z,u)=((-5+4a)/7,(9+11a-b)/7,a,b)
\\a(\frac{4}{7},\frac{11}{7},10)+b(0,-1,0,1)+(-\frac{5}{7},\frac{9}{7},0,0)
$$

(8) 2.21 Pr 7 
$$
\text{If we interchange the rows and columns of a rectangular matrix }A 
\\ \text{ the new matrix so obtained
is called the transpose of }A\text{ and is denoted by }A^t
\\\text{ For example, if we have }
\\ A= \left[ \begin{matrix}1&2&3\\4&5&6 \end{matrix} \right], A^T= \left[ \begin{matrix}1&4\\2&5\\3&6 \end{matrix} \right]
\\ \text{prove following properties}
$$

$$
\text{a) }(A^T)^T=A
\\
\\ \text{if }A \text{ is }n\times m \text{ matrix }A^T \text{ is }m\times n \text{ and } (A^T)^T \text{ is }n\times m \text{ matrix }
\\
\\ (i,j)^{th} \text{element of }(A^T)^T \text{ is } (j,i)^{th} \text{ element of } A^T
\\ (j,i)^{th} \text{element of }A^T \text{ is } (i,j)^{th} \text{ element of } A\
\\ \text{therefore }(i,j)^{th}\text{ element of }(A^T)^T \text{ is equal to }(i,j)^{th}\text{ element of }A
\\
\\ \text{Therefore }(A^T)^T=A
$$

$$
\text{b) } (A + B)^t = A^t + B^t
\\
\\ \text{let }(i,j)^{th}\text{ element of }A \text{ is }a
\\ \text{let }(i,j)^{th}\text{ element of }B \text{ is }b
\\ 
\\ (j,i)^{th}\text{ element of }(A + B)^t \text{ is }(i,j)^{th}\text{ element of }(A + B)
\\(i,j)^{th}\text{ element of }(A + B) \text{ is }a+b
\\
\\ (j,i)^{th}\text{ element of }A^t \text{ and } B^t \text{ are }a \text{ and }b
\\ A^t + B^t=a+b
\\
\\ \text{therefore } (A + B)^t = A^t + B^t
$$

$$
\text{c) }(cA)^t = cA^t
\\
\\ (j,i)^{th}\text{ element of }(cA)^t \text{ is }(i,j)^{th}\text{ element of }cA
\\ \text{Since c is scalar }(i,j)^{th}\text{ element of }cA \text{ is }c\times((i,j)^{th}\text{ element of }A)
\\
\\(j,i)^{th}\text{ element of }cA^t \text{ is }c\times((i,j)^{th}\text{ element of }A)
\\
\\ \text{therefore }(cA)^t = cA^t
$$

$$
\text{d) } (AB)^t = B^tA^t
\\
\\ \text{let }(i,j)^{th}\text{ element of }A \text{ is }a
\\ \text{let }(i,j)^{th}\text{ element of }B \text{ is }b
\\
\\ (j,i)^{th}\text{ element of }(AB)^t \text{ is }(i,j)^{th} \text{element of }AB
\\(i,j)^{th} \text{element of }AB \text{ is equal to }ab
\\
\\ (j,i)^{th}\text{ element of } B^tA^t\text{ is product of } (j,i)^{th}\text{ element of }B^t \text{ and }A^t
\\(j,i)^{th}\text{ element of }B^t \text{ and }A^t \text{ are equal to }a \text{ and }b
\\ B^tA^t=ab
\\
\\ \text{Therefore }(AB)^t = B^tA^t
$$

$$
\text{e) }(A^t)^{-1} = (A^{-1})^t \text{ if A is nonsingular}
\\
\\ \text{in d) we showed that }(AB)^t = B^tA^t
\\ 
\\ (A^t)^{-1} = (A^{-1})^t \text{ on both side we are going to multiply }A^t
\\(A^t)^{-1}A^t=I
\\
\\(A^{-1})^tA^t=(A^{-1}A)^t=(I)t=I \text{ use what we showed in problem d}
\\ 
\\ \text{Therefore }(A^t)^{-1} = (A^{-1})^t 
$$

