# Math 375

### Geonho Roh

**(1) 2.8 Pr 19** 

- Determine one-to-one 
  - Describe its range
  - Find inverse

$$
T(x,y,z)=(x,x+y,x+y+z)
$$

$$
\text{ Check one-to-one}
\\ \text{Let }A=(x_1,y_1,z_1) \ B=(x_2,y_2,z_2)
\\ \text{If it is one-to-one it must follow }T(A)=T(B) \text{ then } A=B
\\
\\ T(A)=T(B)
\\ (x_1,x_1+y_1,x_1+y_1+z_1)=(x_2,x_2+y_2,x_2+y_2+z_2)
\\\\ x_1=x_2
\\ x_1+y_1=x_2+y_2
\\x_1+y_1+z_1=x_2+y_2+z_2
$$

$$
\text{Solving the equation we get}
\\ x_1=x_2, y_1=y_2, z_1=z_2
\\ \text{So } A= B
\\ \text{Therefore it is one-to-one}
\\ 
\\ x(1,1,1)+y(0,1,1)+z(0,0,1)=(x,x+y,x+y+z)
\\ (1,1,1),(0,1,1),(0,0,1) \text{ form a basis for range of } T 
\\ \text{The Range is } \R^3
\\
\\ T(x,y,z)=(u,v,w)
\\ (x,x+y,x+y+z)=(u,v,w)
\\ x=u,y=v-u,z=w-v
\\ T^{-1}(u,v,w)=(x,y,z)
\\T^{-1}(u,v,w)=(u,v-u,w-v)
\\
\\ \text{Check }TT^{-1}(x,y,z)=(x,y,z)
\\ T(x,y-x,z-y)=(x,x+y-x,z+y-x+z-y)=(x,y,z)
$$

$$
\text{Answer) It is one-to-one }
\\ \text{Spanned by }(1,1,1),(0,1,1),(0,0,1) \text{ which is }\R^3
\\ T^{-1}(u,v,w)=(u,v-u,w-v)
$$

(2) 2.8 Pr 22
$$
\text{If S and T commute, prove that} (ST)^n = S^nT^n \text{ for all integers }n \geq0
$$

$$
\\ \text{Before proving for the }(ST)^n = S^nT^n \text{ we are going to show for } ST^n=T^nS
\\ \text{It is trivial for }n=0 \text{ Since }T^0 = I
\\ \text{ for }n=1 \text{ it is true because }ST^1=ST=TS
\\ \text{Assume it is true for n and prove for n+1}
\\ 
\\ ST^{n+1}=STT^n
\\=TST^n \text{ since we assume it is true for }n
\\=TT^nS
\\ =T^{n+1}S
\\
\\ \text{It is true for n+1 therefore it is true}
$$

$$
\\ \text{Prove }(ST)^n = S^nT^n \text{ for all integers }n \geq0
\\
\\\text{It is trivial for }n=0 \text{ Since }T^0 = I
\\ 
\text{ for }n=1 \text{ it is true because }(ST)^1=S^1T^1
\\ \text{Assume it is true for }n \text{ prove for }n+1
\\ 
\\ \text{For }n+1\ \ (ST)^{n+1}=(ST)^n(ST)=S^nT^n(ST)
\\ \text{Since they commute }S^nT^n(ST)=S^nST^nT=S^{n+1}T^{n+1} \text{  (use what we proved in previous induction)}
\\ (ST)^{n+1}=S^{n+1}T^{n+1} \text{ is true}
\\
\\ \text{Therefore statement }(ST)^n = S^nT^n \text{ for all integers }n \geq0 \text{ is true}
$$



(3) 2.8 Pr 24
$$
\text{If S and Tare invertible and commute, prove that their inverses also commute.}
$$

$$
ST=TS \text{ and }S^{-1} \ T^{-1} \text{ exist}
\\ 
\\ ST=TS
\\ S^{-1}ST=S^{-1}TS
\\ IT=S^{-1}TS
\\T=S^{-1}TS
\\ T^{-1}T=T^{-1}S^{-1}TS
\\I=T^{-1}S^{-1}TS
\\ IS^{-1}=T^{-1}S^{-1}TSS^{-1}
\\ S^{-1}=T^{-1}S^{-1}TI
\\S^{-1}T^{-1}=T^{-1}S^{-1}TT^{-1}
\\S^{-1}T^{-1}=T^{-1}S^{-1}I
\\S^{-1}T^{-1}=T^{-1}S^{-1}
\\
\\ \text{Therefore inverse is also commute}
$$

(4) 2.12 Pr 3
$$
\text{A linear transformation } T: V_2 \rightarrow 	V_2, \text{maps the basis vectors i andj as follows:}
\\ T(i)=i+j \ \ \ T(j)=2i-j
$$

$$
\text{a) Compute } T(3i - 4j) \text{ and }T^2(3i - 4j) \text{ in terms of i and j.}
\\
\\ \text{Since it is a linear transformation it must follow}
\\ T(a\alpha+b\beta)=aT(\alpha)+bT(\beta) \text{ where } \alpha,\beta \in V_2 \text{ and scalars }a,b
\\\\
\\ T(3i-4j)=3T(i)-4T(j)=3(i+j)-4(2i-j)=-5i+7j
\\
\\T^2(3i - 4j)=TT(3i-4j)=T(-5i+7j)
\\=-5T(i)+7T(j)=-5(i+j)+7(2i-j)=9i-12j
$$

$$
\text{b) Determine the matrix of } T\text{ and }T^2
\\ \text{basis is }(i,j)
\\ T(i)=(1)i+(1)j, \ \ T(j)=(2)i+(-1)j
\\ T(i)=\left[ \begin{matrix} 1 \\1 \end{matrix} \right], T(j)=\left[ \begin{matrix} 2 \\-1 \end{matrix} \right]
\\ \text{So }[T]=\left[ \begin{matrix} 1 & 2\\1&-1\end{matrix} \right]
\\ 
\\ T^2 =\left[ \begin{matrix} 1 & 2\\1&-1\end{matrix} \right]\left[ \begin{matrix} 1 & 2\\1&-1\end{matrix} \right]=\left[ \begin{matrix} 3 & 0\\0&3\end{matrix} \right]
$$

$$
\text{c) Solve b if basis is replaced by }(e_1,e_2) \ \ e_1=i-j, e_2=3i+j
\\
\\T(e_1)=T(i-j)=-i+2j = a(i-j)+b(3i+j) \ \ \text{ using problem a}
\\
\\a+3b=-1
\\-a+b=2
\\ a=\frac{-7}{4},b=\frac{1}{4}
\\ \text{So }T(e_1)=\left[ \begin{matrix} \frac{-7}{4}\\\frac{1}{4}\end{matrix} \right]
\\
\\T(e_2)=T(3i+j)=5i+2j=a(i-j)+b(3i+j) \ \ \text{ using problem a}
\\a+3b=5
\\-a+b=2
\\a= \frac{-1}{4},b=\frac{7}{4}
\\ \text{So }T(e_2)=\left[ \begin{matrix} \frac{-1}{4}\\\frac{7}{4}\end{matrix} \right]
\\
\\ [T]=\left[ \begin{matrix} \frac{-7}{4}&\frac{-1}{4}\\\frac{1}{4}&\frac{7}{4}\end{matrix} \right]
\\
\\T^2=\left[ \begin{matrix} \frac{-7}{4}&\frac{-1}{4}\\\frac{1}{4}&\frac{7}{4}\end{matrix} \right]\left[ \begin{matrix} \frac{-7}{4}&\frac{-1}{4}\\\frac{1}{4}&\frac{7}{4}\end{matrix} \right]=\left[ \begin{matrix} 3&0\\0&3\end{matrix} \right]
$$



(5) 2.12 Pr 8
$$
\text{A linear transformation }T: V_2\rightarrow V_3\text{ maps the basis vectors as follows: } T(i) = (1, 0,1), T(j)=(-1,0,1)
$$

$$
\text{a)  Compute }T(2i - 3j)\text{ and determine the nullity and rank of T.}
\\
\\ \text{Since it is a linear transformation it must follow}
\\ T(a\alpha+b\beta)=aT(\alpha)+bT(\beta) \text{ where } \alpha,\beta \in V_2 \text{ and scalars }a,b
\\
\\T(2i - 3j)=2T(i)-3T(j)=2(1, 0,1)-3(-1,0,1)=(5,0,-1)
\\
\\ \text{Representative matrix of T }
\\ T(i)=(1,0,1)=1(1,0,0)+0(0,1,0)+1(0,0,1)
\\ T(j)=(-1,0,1)=-1(1,0,0)+0(0,1,0)+1(0,0,1)
\\
\\ [T]=\left[ \begin{matrix} 1&-1\\0&0 \\ 1&1\end{matrix} \right]
\\ \text{So }T(v) ,v=\left[ \begin{matrix}x_1\\x_2\end{matrix} \right] v \in V_2 
\\T(v)=\left[ \begin{matrix} 1&-1\\0&0 \\ 1&1\end{matrix} \right]\left[ \begin{matrix}x_1\\x_2\end{matrix} \right] =\left[ \begin{matrix}x_1-x_2\\0\\x_1+x_2\end{matrix} \right] 
\\
\\ \text{The nullity of T }
\\\text{When }x_1=0, x_2=0
\\ \left[ \begin{matrix}x_1-x_2\\0\\x_1+x_2\end{matrix} \right] =\left[ \begin{matrix}0\\0\\0\end{matrix} \right]
\\\text{Therefore nullity of T is }0
\\
\\ \text{Range of T is spanned by }\left[ \begin{matrix} 1&-1\\0&0 \\ 1&1\end{matrix} \right]
\\ \text{Rank is }2
$$

$$
\text{b) Determine the matrix of }T
\\
\\ \text{In part a we showed the matrix of T}
\\ [T]=\left[ \begin{matrix} 1&-1\\0&0 \\ 1&1\end{matrix} \right]
$$

$$
\text{c) Find bases } (e_1, e_2) \text{ for } V_2 \text{ and } (w_1, w_2, w_3)\text{ for } V_3 \text{ relative to which the matrix of } T \text{ will be in diagonal form.}
\\
\\ \text{let }e_1=i,e_2=j
\\ w_1=\left[ \begin{matrix}1\\0\\1\end{matrix} \right],w_2=\left[ \begin{matrix}-1\\0\\1\end{matrix} \right],w_3=\left[ \begin{matrix}0\\1\\0\end{matrix} \right]
\\
\\ T(e_1)=a_1w_1+a_2w_2+a_3w_3
\\ T(e_2)=b_1w_1+b_2w_2+b_3w_3
\\ \text{to be a diagonal form }a_2=a_3=0, b_1=b_3=0
\\ T(e_1)=a_1w_1
\\ T(e_2)=b_2w_2
\\
\\T(e_1)=\left[ \begin{matrix}1\\0\\1\end{matrix} \right]=a\left[ \begin{matrix}1\\0\\1\end{matrix} \right]
\\T(e_2)=\left[ \begin{matrix}-1\\0\\1\end{matrix} \right]=b\left[ \begin{matrix}-1\\0\\1\end{matrix} \right]
\\
\\ \text{Since }a=b=1 \text{ matrix of T in a diagonal form is made} 
\\ [T]=\left[ \begin{matrix}1&0\\0&1\\0&0\end{matrix} \right] 
\\
\\e_1=i,e_2=j
\\ w_1=\left[ \begin{matrix}1\\0\\1\end{matrix} \right],w_2=\left[ \begin{matrix}-1\\0\\1\end{matrix} \right],w_3=\left[ \begin{matrix}0\\1\\0\end{matrix} \right]
$$

(6) 2.16 Pr 1
$$
\text{If }A=\left[ \begin{matrix}1&-4&2\\-1&4&-2\end{matrix} \right],B=\left[ \begin{matrix}1&2\\-1&3\\5&-2\end{matrix} \right],C=\left[ \begin{matrix}2&2\\1&-1\\1&-3\end{matrix} \right]
\\ \text{Compute }B+C,AB,BA,AC,CA,A(2B-3C)
\\
\\ B+C
\\ = \left[ \begin{matrix}1&2\\-1&3\\5&-2\end{matrix} \right]+\left[ \begin{matrix}2&2\\1&-1\\1&-3\end{matrix} \right]
\\ =\left[ \begin{matrix}1+2&2+2\\-1+1&3-1\\5+1&-2-3\end{matrix} \right]
\\ =\left[ \begin{matrix}3&4\\0&2\\6&-5\end{matrix} \right]
$$

$$
AB
\\ =\left[ \begin{matrix}1&-4&2\\-1&4&-2\end{matrix} \right]\left[ \begin{matrix}1&2\\-1&3\\5&-2\end{matrix} \right]
\\=\left[ \begin{matrix}1+4+10&2-12-4\\-1-4-10&-2+12+4\end{matrix} \right]=\left[ \begin{matrix}15&-14\\-15&14\end{matrix} \right]
\\
\\BA
\\ =\left[ \begin{matrix}1&2\\-1&3\\5&-2\end{matrix} \right]\left[ \begin{matrix}1&-4&2\\-1&4&-2\end{matrix} \right]
\\=\left[ \begin{matrix}1-2&-4+8&2-4\\-1-3&4+12&-2-6\\5+2&-20-8&10+4\end{matrix} \right]=\left[ \begin{matrix}-1&4&-2\\-4&16&-8\\7&-28&14\end{matrix} \right]
$$

$$
AC
\\ =\left[ \begin{matrix}1&-4&2\\-1&4&-2\end{matrix} \right]\left[ \begin{matrix}2&2\\1&-1\\1&-3\end{matrix} \right]
\\ = \left[ \begin{matrix}2-4+2&2+4-6\\-2+4-2&-2-4+6\end{matrix} \right]=\left[ \begin{matrix}0&0\\0&0\end{matrix} \right]
\\
\\ CA
\\=\left[ \begin{matrix}2&2\\1&-1\\1&-3\end{matrix} \right]\left[ \begin{matrix}1&-4&2\\-1&4&-2\end{matrix} \right]
\\=\left[ \begin{matrix}2-2&-8+8&4-4\\1+1&-4-4&2+2\\1+3&-4-12&2+6\end{matrix} \right]=\left[ \begin{matrix}0&0&0\\2&-8&4\\4&-16&8\end{matrix} \right]
\\
$$

$$
\\A(2B-3C)
\\=\left[ \begin{matrix}1&-4&2\\-1&4&-2\end{matrix} \right](2\left[ \begin{matrix}1&2\\-1&3\\5&-2\end{matrix} \right]-3\left[ \begin{matrix}2&2\\1&-1\\1&-3\end{matrix} \right])
\\=\left[ \begin{matrix}1&-4&2\\-1&4&-2\end{matrix} \right]\left[ \begin{matrix}2-6&4-6\\-2-3&6+3\\10-3&-4+9\end{matrix} \right]
\\=\left[ \begin{matrix}1&-4&2\\-1&4&-2\end{matrix} \right]\left[ \begin{matrix}-4&-2\\-5&9\\7&5\end{matrix} \right]
\\=\left[ \begin{matrix}-4+20+14&-2-36+10\\4-20-14&2+36-10\end{matrix} \right]
\\=\left[ \begin{matrix}30&-28\\-30&28\end{matrix} \right]
$$

(7) 2.16 Pr 3
$$
\text{find }a,b,c,d
$$

$$
\left[ \begin{matrix}0&0&1&0\\1&0&0&0\\0&1&0&0\\0&0&0&1\end{matrix} \right]\left[ \begin{matrix}a\\b\\c\\d\end{matrix} \right]=\left[ \begin{matrix}1\\9\\6\\5\end{matrix} \right]
\\
\\\left[ \begin{matrix}0&0&1&0\\1&0&0&0\\0&1&0&0\\0&0&0&1\end{matrix} \right]\left[ \begin{matrix}a\\b\\c\\d\end{matrix} \right]=\left[ \begin{matrix}c\\a\\b\\d\end{matrix} \right]
\\ \left[ \begin{matrix}c\\a\\b\\d\end{matrix} \right]=\left[ \begin{matrix}1\\9\\6\\5\end{matrix} \right]
\\a=9,b=6,c=1,d=5
$$

$$
\left[ \begin{matrix}a&b&c&d\\1&4&9&2\end{matrix} \right]\left[ \begin{matrix}1&0&2&0\\0&0&1&1\\0&1&0&0\\0&0&1&0\end{matrix} \right]=\left[ \begin{matrix}1&0&6&6\\1&9&8&4\end{matrix} \right]
\\
\\\left[ \begin{matrix}a&b&c&d\\1&4&9&2\end{matrix} \right]\left[ \begin{matrix}1&0&2&0\\0&0&1&1\\0&1&0&0\\0&0&1&0\end{matrix} \right]=\left[ \begin{matrix}a&c&2a+b+d&b\\1&9&2+4+2&4\end{matrix} \right]
\\\left[ \begin{matrix}a&c&2a+b+d&b\\1&9&8&4\end{matrix} \right]=\left[ \begin{matrix}1&0&6&6\\1&9&8&4\end{matrix} \right]
\\
\\ a=1,c=0,2a+b+d=6,b=6
\\ \text{Solving the equation}
\\
\\a=1,b=6,c=0,d=-2
$$

(8) 2.16 Pr 4
$$
\text{Calculate }AB-BA \text{ in each case}
$$

$$
A=\left[ \begin{matrix}1&2&2\\2&1&2\\1&2&3\end{matrix} \right] ,B=\left[ \begin{matrix}4&1&1\\-4&2&0\\1&2&1\end{matrix} \right]
\\
\\AB
\\=\left[ \begin{matrix}1&2&2\\2&1&2\\1&2&3\end{matrix} \right]\left[ \begin{matrix}4&1&1\\-4&2&0\\1&2&1\end{matrix} \right]
\\= \left[ \begin{matrix}4-8+2&1+4+4&1+0+2\\8-4+2&2+2+4&2+0+2\\4-8+3&1+4+6&1+0+3\end{matrix} \right]
\\=\left[ \begin{matrix}-2&9&3\\6&8&4\\-1&11&4\end{matrix} \right]
\\
\\BA
\\=\left[ \begin{matrix}4&1&1\\-4&2&0\\1&2&1\end{matrix} \right]\left[ \begin{matrix}1&2&2\\2&1&2\\1&2&3\end{matrix} \right]
\\= \left[ \begin{matrix}4+2+1&8+1+2&8+2+3\\-4+4+0&-8+2+0&-8+4+0\\1+4+1&2+2+2&2+4+3\end{matrix} \right]
\\=\left[ \begin{matrix}7&11&13\\0&-6&-4\\6&6&9\end{matrix} \right]
$$

$$
\\AB-BA=\left[ \begin{matrix}-2&9&3\\6&8&4\\-1&11&4\end{matrix} \right]-\left[ \begin{matrix}7&11&13\\0&-6&-4\\6&6&9\end{matrix} \right]
\\=\left[ \begin{matrix}-2-7&9-11&3-13\\6-0&8-(-6)&4-(-4)\\-1-6&11-6&4-9\end{matrix} \right]
\\=\left[ \begin{matrix}-9&-2&-10\\6&14&8\\-7&5&-5\end{matrix} \right]
$$

----

$$
A=\left[ \begin{matrix}2&0&0\\1&1&2\\-1&2&1\end{matrix} \right] ,B=\left[ \begin{matrix}3&1&-2\\3&-2&4\\-3&5&11\end{matrix} \right]
\\
\\AB
\\=\left[ \begin{matrix}2&0&0\\1&1&2\\-1&2&1\end{matrix} \right]\left[ \begin{matrix}3&1&-2\\3&-2&4\\-3&5&11\end{matrix} \right]
\\= \left[ \begin{matrix}6+0+0&2+0+0&-4+0+0\\3+3-6&1-2+10&-2+4+22\\-3+6-3&-1-4+5&2+8+11\end{matrix} \right]
\\=\left[ \begin{matrix}6&2&-4\\0&9&24\\0&0&21\end{matrix} \right]
\\
\\BA
\\=\left[ \begin{matrix}3&1&-2\\3&-2&4\\-3&5&11\end{matrix} \right]\left[ \begin{matrix}2&0&0\\1&1&2\\-1&2&1\end{matrix} \right]
\\= \left[ \begin{matrix}6+1+2&0+1-4&0+2-2\\6-2-4&0-2+8&0-4+4\\-6+5-11&0+5+22&0+10+11\end{matrix} \right]
\\=\left[ \begin{matrix}9&-3&0\\0&6&0\\-12&27&21\end{matrix} \right]
$$

$$
AB-BA=\left[ \begin{matrix}6&2&-4\\0&9&24\\0&0&21\end{matrix} \right]-\left[ \begin{matrix}9&-3&0\\0&6&0\\-12&27&21\end{matrix} \right]
\\ =\left[ \begin{matrix}6-9&2-(-3)&-4-0\\0-0&9-6&24-0\\0-(-12)&0-27&21-21\end{matrix} \right]
\\=\left[ \begin{matrix}-3&5&-4\\0&3&24\\12&-27&0\end{matrix} \right]
$$

