# Math 375

#### Geonho Roh

(1) 3.6 Pr 1 
$$
\text{Compute each of the following determinants}
$$

$$
\text{a) }\begin{bmatrix}2&1&1 \\ 1&4&-4\\1&0&2  \end{bmatrix}
\\
\\ \text{Using upper trianglular form}
\\ \begin{bmatrix}2&1&1 \\ 1&4&-4\\1&0&2  \end{bmatrix} \rightarrow\begin{bmatrix}2&1&1 \\ 0&4&-6\\1&0&2  \end{bmatrix}\rightarrow\begin{bmatrix}2&1&1 \\ 0&4&-6\\0&-\frac{1}{2}&\frac{3}{2}  \end{bmatrix}
\\ \rightarrow\begin{bmatrix}2&1&1 \\ 0&4&-6\\0&0&\frac{3}{4}   \end{bmatrix}
\\ 
\\ det =2\times6\times\frac{3}{4} = 6
$$

---

$$
\text{b) }\begin{bmatrix}3&0&8 \\ 5&0&7\\-1&4&2  \end{bmatrix}
\\
\\ \text{using upper triangular form}
\\ \begin{bmatrix}3&0&8 \\ 5&0&7\\-1&4&2  \end{bmatrix}\rightarrow\begin{bmatrix}3&0&8 \\ 0&20&17\\-1&4&2  \end{bmatrix} \rightarrow (\times 3 \text{ det})\begin{bmatrix}3&0&8 \\ 0&20&17\\-3&12&6  \end{bmatrix}
\\ \rightarrow \begin{bmatrix}3&0&8 \\ 0&20&17\\0&12&14  \end{bmatrix}\rightarrow \begin{bmatrix}3&0&8 \\ 0&20&17\\0&0&14-\frac{3}{5}17  \end{bmatrix}
\\
\\ det = \frac{1}{3}\times3\times20\times(14-\frac{51}{5} )=280-204=76
$$

-----

$$
\text{c) }\begin{bmatrix}a&1&0 \\ 2&a&2\\0&1&a  \end{bmatrix}
\\
\\ \text{using equation 3.2}
\\ \det = a \ \det\begin{bmatrix}a&2 \\ 1&a \end{bmatrix}-1\ \det\begin{bmatrix}2&2 \\ 0&a \end{bmatrix}+ 0 \det \begin{bmatrix}2&a \\ 0&1 \end{bmatrix}
\\ = a(a^2-2)-1(2a-0)=a^3-4a
$$

(2) 3.6 Pr 2 
$$
\text{If determinant of }\begin{bmatrix}x&y&z \\ 3&0&2\\1&1&1 \end{bmatrix} =1 \text{ compute the determinant of following matrices}
$$

$$
\\ \begin{bmatrix}x&y&z \\ 3&0&2\\1&1&1 \end{bmatrix}
\\
\\ \\ \det \begin{bmatrix}x&y&z \\ 3&0&2\\1&1&1 \end{bmatrix} = x\ \det\begin{bmatrix}0&2 \\ 1&1 \end{bmatrix}-y \det\begin{bmatrix}3&2 \\ 1&1 \end{bmatrix}+z\det\begin{bmatrix}3&0 \\ 1&1 \end{bmatrix}
\\ = x(-2)-y(3-2)+z(3-0)
\\=-2x-y+3z
$$


$$
\text{a) }\det \begin{bmatrix}2x&2y&2z \\ 3/2&0&1\\1&1&1 \end{bmatrix}=\det2\begin{bmatrix}x&y&z \\ 3/2&0&1\\1&1&1 \end{bmatrix}=\det\begin{bmatrix}x&y&z \\ 3&0&2\\1&1&1 \end{bmatrix}=1
$$

---

$$
\text{b) }\begin{bmatrix}x&y&z \\ 3x+3&3y&3z+2\\x+1&y+1&z+1 \end{bmatrix}
\\
\\ \det\begin{bmatrix}x&y&z \\ 3x+3&3y&3z+2\\x+1&y+1&z+1 \end{bmatrix}=\det\begin{bmatrix}x&y&z \\ 3&0&2\\x+1&y+1&z+1 \end{bmatrix}=\det\begin{bmatrix}x&y&z \\ 3&0&2\\x+1&y+1&z+1 \end{bmatrix}
\\=\det\begin{bmatrix}x&y&z \\ 3&0&2\\1&1&1 \end{bmatrix}=1
$$

---

$$
\text{c) }\begin{bmatrix}x-1&y-1&z-1 \\ 4&1&3\\1&1&1 \end{bmatrix}
\\
\\\det\begin{bmatrix}x-1&y-1&z-1 \\ 4&1&3\\1&1&1 \end{bmatrix}=\det\begin{bmatrix}x&y&z \\ 4&1&3\\1&1&1 \end{bmatrix}
\\=\det\begin{bmatrix}x&y&z \\ 3&0&2\\1&1&1 \end{bmatrix}=1
$$

(3) 3.11 Pr 1 
$$
\text{ For each of the following statements about square matrices, give a proof or exhibit a counter
example}
$$

$$
\text{a) } \det A+\det B=\det(A+B)
\\
\\ \text{Not true}
\\ A=\begin{bmatrix}1&0 \\ 0&1 \end{bmatrix}, B=\begin{bmatrix}2&0 \\ 0&2 \end{bmatrix}
\\ \det A=1, \det B=4
\\ \det(A+B)=\det\begin{bmatrix}3&0 \\ 0&3 \end{bmatrix}=9
$$

----

$$
\text{b) }\det((A+B)^2)=(\det(A+B))^2
\\
\\\det((A+B)^2)=\det((A+B)(A+B))
\\ \text{Since }\det AB=\det A\det B
\\ \det((A+B)(A+B))=\det(A+B)\det(A+B)=(\det(A+B))^2
$$

---

$$
\text{c) }\det((A+B)^2)=\det(A^2+2AB+B^2)
\\
\\ \text{For the equation to be true}
\\ (A+B)(A+B)=A^2+BA+AB+B^2=A^2+2AB+B^2
\\ \text{It has to satisfy }AB=BA
\\
\\ \text{However it is false since counter Ex exist}
\\ A =\begin{bmatrix}1&1 \\ 0&1 \end{bmatrix}, B=\begin{bmatrix}1&0 \\ 1&0 \end{bmatrix}
\\ AB=\begin{bmatrix}1&1 \\ 0&1 \end{bmatrix}\begin{bmatrix}1&0 \\ 1&0 \end{bmatrix}=\begin{bmatrix}2&0 \\ 1&0 \end{bmatrix}
\\ BA=\begin{bmatrix}1&0 \\ 1&0 \end{bmatrix}\begin{bmatrix}1&1 \\ 0&1 \end{bmatrix}=\begin{bmatrix}1&1 \\ 1&1 \end{bmatrix}
$$

---

$$
\text{d) }\det((A+B)^2)=\det(A^2+B^2)
\\
\\ \text{If }\det((A+B)^2)=\det(A^2+B^2) 
\\ AB+BA = 0
\\ \text{Using the process from previous question we can easily check that }
\\ AB+BA \neq 0
$$

(4) 3.17 Pr 1 

$$
\text{Determine the cofactor of following matrices}
\\
$$

$$
\text{a) }\begin{bmatrix}1&2 \\ 3&4 \end{bmatrix}
\\
\\ cof(a_{11})=(-1)^{1+1}4=4
\\ cof(a_{12})=(-1)^{1+2}3=-3
\\ cof(a_{21})=(-1)^{2+1}2=-2
\\ cof(a_{22})=(-1)^{2+2}1=1
\\
\\ \begin{bmatrix}4&-3 \\ -2&1 \end{bmatrix}
$$

---

$$
\text{b) }\begin{bmatrix}2&-1&3\\0&1&1 \\ -1&-2&0 \end{bmatrix}
\\
\\ cof(a_{11})=(-1)^{1+1}\det\begin{bmatrix}1&1 \\ -2&0 \end{bmatrix}=2
\\ cof(a_{12})=(-1)^{1+2}\det\begin{bmatrix}0&1 \\ -1&0 \end{bmatrix}=-1
\\ cof(a_{13})=(-1)^{1+3}\det\begin{bmatrix}0&1 \\ -1&-2 \end{bmatrix}=1
\\ cof(a_{21})=(-1)^{2+1}\det\begin{bmatrix}-1&3 \\ -2&0 \end{bmatrix}=-6
\\ cof(a_{22})=(-1)^{2+2}\det\begin{bmatrix}2&3 \\ -1&0 \end{bmatrix}=3
\\ cof(a_{23})=(-1)^{2+3}\det\begin{bmatrix}2&-1 \\ -1&-2 \end{bmatrix}=5
\\ cof(a_{31})=(-1)^{3+1}\det\begin{bmatrix}-1&3 \\ 1&1 \end{bmatrix}=-4
\\ cof(a_{32})=(-1)^{3+2}\det\begin{bmatrix}2&3 \\ 0&1 \end{bmatrix}=-2
\\ cof(a_{33})=(-1)^{3+3}\det\begin{bmatrix}2&-1 \\ 0&1 \end{bmatrix}=2
\\
\\ \begin{bmatrix}2&-1&1 \\ -6&3&5 \\-4&-2&2\end{bmatrix}
$$

----

$$
\text{c) } \begin{bmatrix}3&1&2&4 \\ 2&0&5&1\\1&-1&-2&6 \\ -2&3&2&3\end{bmatrix}
\\
\\ cof(a_{11})= (-1)^{1+1}\det\begin{bmatrix} 0&5&1\\-1&-2&6 \\ 3&2&3\end{bmatrix}=(-1)^{1+1}((-5)(-21)+1(4))=109
\\ cof(a_{12})= (-1)^{1+2}\det\begin{bmatrix} 2&5&1\\1&-2&6 \\ -2&2&3\end{bmatrix}=(-1)^{1+2}((2)(-18)+(-5)(15)+1(-2))=113
\\ cof(a_{13})= (-1)^{1+3}\det\begin{bmatrix} 2&0&1\\1&-1&6 \\ -2&3&3\end{bmatrix}=(-1)^{1+3}((2)(-21)+1(1))=-41
\\ cof(a_{14})= (-1)^{1+4}\det\begin{bmatrix} 2&0&5\\1&-1&-2 \\ -2&3&2\end{bmatrix}=(-1)^{1+4}((2)(4)+5(1))=-13
\\
\\ cof(a_{21})= (-1)^{2+1}\det\begin{bmatrix} 1&2&4\\-1&-2&6 \\3&2&3\end{bmatrix}=(-1)^{2+1}((1)(-18)+(-2)(-21)+4(4))=-40
\\ cof(a_{22})= (-1)^{2+2}\det\begin{bmatrix} 3&2&4\\1&-2&6 \\ -2&2&3\end{bmatrix}=(-1)^{2+2}((3)(-18)+(-2)15+4(-2))=-92
\\ cof(a_{23})= (-1)^{2+3}\det\begin{bmatrix} 3&1&4\\1&-1&6 \\ -2&3&3\end{bmatrix}=(-1)^{2+3}((3)(-21)+(-1)15+4(1))=74
\\ cof(a_{24})= (-1)^{2+4}\det\begin{bmatrix} 3&1&2\\1&-1&-2 \\ -2&3&2\end{bmatrix}=(-1)^{2+4}((3)(4)+(-1)(-2)+2(1))=16
\\
$$

$$
\text{c) } \begin{bmatrix}3&1&2&4 \\ 2&0&5&1\\1&-1&-2&6 \\ -2&3&2&3\end{bmatrix}
\\
\\ cof(a_{31})= (-1)^{3+1}\det\begin{bmatrix} 1&2&4\\0&5&1 \\ 3&2&3\end{bmatrix}=(-1)^{3+1}((1)(13)+(-2)(-3)+4(-15))=-41
\\ cof(a_{32})= (-1)^{3+2}\det\begin{bmatrix} 3&2&4\\2&5&1 \\ -2&2&3\end{bmatrix}=(-1)^{3+2}((3)(13)+(-2)8+4(14))=-79
\\ cof(a_{33})= (-1)^{3+3}\det\begin{bmatrix} 3&1&4\\2&0&1 \\ -2&3&3\end{bmatrix}=(-1)^{3+3}((3)(-3)+(-1)8+4(6))=7
\\ cof(a_{34})= (-1)^{3+4}\det\begin{bmatrix} 3&1&2\\2&0&5 \\ -2&3&2\end{bmatrix}=(-1)^{3+4}((3)(-15)+(-1)14+2(6))=47
\\
\\ cof(a_{41})= (-1)^{4+1}\det\begin{bmatrix} 1&2&4\\0&5&1 \\ -1&-2&6\end{bmatrix}=(-1)^{4+1}((1)(32)+(-2)(1)+4(5))=-50
\\ cof(a_{42})= (-1)^{4+2}\det\begin{bmatrix} 3&2&4\\2&5&1 \\ 1&-2&6\end{bmatrix}=(-1)^{4+2}((3)(32)+(-2)11+4(-9))=38
\\ cof(a_{43})= (-1)^{4+3}\det\begin{bmatrix} 3&1&4\\2&0&1 \\ 1&-1&6\end{bmatrix}=(-1)^{4+3}((3)(1)+(-1)11+4(-2))=16
\\ cof(a_{44})= (-1)^{4+4}\det\begin{bmatrix} 3&1&2 \\ 2&0&5 \\ 1&-1&-2\end{bmatrix}=(-1)^{1+1}((3)(5)+(-1)(-9)+2(-2))=20
\\
\\ \begin{bmatrix}109&113&-41&-13 \\ -40&-92&74&16\\-41&-79&7&47 \\ -50&38&16&20\end{bmatrix}
$$

(5) 3.17 Pr 3 
$$
\text{Find all values of the scalar }\lambda \text{ for which the matrix } \lambda I \ - A \text{ is singular, if A is equal to}
$$

$$
\text{a) }A = \begin{bmatrix}0&3 \\ 2&-1 \end{bmatrix}
\\
\\ \lambda I - A = \begin{bmatrix}\lambda&0 \\ 0&\lambda \end{bmatrix}-\begin{bmatrix}0&3 \\ 2&-1 \end{bmatrix}
\\ = \begin{bmatrix}\lambda&-3\\ -2&\lambda+1 \end{bmatrix} 
\\
\\ \text{to be singular }\det\begin{bmatrix}\lambda&-3\\ -2&\lambda+1 \end{bmatrix}=0
\\ \lambda^2+\lambda-6=(\lambda+3)(\lambda-2)
\\
\\ -3,2
$$
------
$$
\text{b) }A=\begin{bmatrix} 1&0&2 \\ 0&-1&-2 \\ 2&-2&0\end{bmatrix}
\\
\\ \lambda I - A = \begin{bmatrix}\lambda&0&0 \\ 0&\lambda&0 \\ 0&0&\lambda \end{bmatrix}-\begin{bmatrix} 1&0&2 \\ 0&-1&-2 \\ 2&-2&0\end{bmatrix}
\\=\begin{bmatrix}\lambda-1&0&-2 \\ 0&\lambda+1&2 \\ -2&2&\lambda \end{bmatrix}
\\
\\\det\begin{bmatrix}\lambda-1&0&-2 \\ 0&\lambda+1&2 \\ -2&2&\lambda \end{bmatrix}=0
\\ \lambda-1(\lambda^2+\lambda-4)-2(2\lambda+2)
\\ = \lambda^3+\lambda^2-4\lambda-\lambda^2-\lambda+4-4\lambda-4
\\=\lambda^3-9\lambda^2
\\
\\ 0,3,-3
$$

---

$$
\text{c) }A=\begin{bmatrix} 11&-2&8 \\ 19&-3&14 \\ -8&2&-5\end{bmatrix}
\\
\\\lambda I - A = \begin{bmatrix}\lambda&0&0 \\ 0&\lambda&0 \\ 0&0&\lambda \end{bmatrix}-\begin{bmatrix} 11&-2&8 \\ 19&-3&14 \\ -8&2&-5\end{bmatrix}
\\=\begin{bmatrix}\lambda-11&2&-8 \\ -19&\lambda+3&-14 \\ 8&-2&\lambda+5 \end{bmatrix}=0

\\
\\ \det\begin{bmatrix}\lambda-11&2&-8 \\ -19&\lambda+3&-14 \\ 8&-2&\lambda+5 \end{bmatrix}=0
\\\lambda-11(\lambda^2+8\lambda+15-28)-2(-19\lambda-95+112)-8(38-8\lambda-24)
\\=\lambda^3+8\lambda^2+15\lambda-28\lambda-11\lambda^2-88\lambda+143+38\lambda-34-112+64\lambda
\\=\lambda^3-3\lambda^2+\lambda-3
\\
\\ 3,i,-i
$$

(6) 4.4 Pr 1 
$$
\text{a) If }\ T\text{ has an eigenvalue }\lambda\text{, prove that }aT \text{ has the eigenvalue }a\lambda
\\
\\ Tx=\lambda x
\\ aTx=a\lambda x
\\ (aT)x=(a\lambda) x
$$

---

$$
\text{b) ) If } x\text{ is an eigenvector for both } T_1 \text{ and }T_2 
\\ \text{ prove that }x \text{ is also an eigenvector for }aT_1 + bT_2
\\\text{How are the eigenvalues related?}
\\
\\ T_1x=\lambda_1x
\\ T_2x=\lambda_2x
\\
\\ aT_1x+bT_2x=a\lambda_1x+b\lambda_2x=(a\lambda_1+b\lambda_2)x
$$

(7) 4.4 Pr 2 1
$$
\text{Assume }T:V\rightarrow V \text{ has an eigenvector }x \text{ belonging to an eigenvalue }\lambda 
\\ \text{Prove that }x\text{ is an eigenvector of }T^2 \text{ belonging to }\lambda^2 \text{ and more generally}
\\x \text{ is an eigenvector of }T^n \text{ belonging to }\lambda^n
\\ \text{Then use the result from Exercise 1 to show that if }P \text{ is a polynomial}
\\ \text{then }x \text{ is an eigenvector of }P(T)\text{ belonging to }P(\lambda)
\\
\\
\\ Tx=x\lambda 
\\ Txx^{-1}= x \lambda x^{-1}
\\ T = x \lambda x^{-1}
\\ T^2 = x \lambda x^{-1}x \lambda x^{-1}=x \lambda^2 x^{-1}
\\ T^2x=x \lambda^2 x^{-1}x=x \lambda^2
\\ 
\\ \text{Using induction }
\\ \text{if }T^nx=x \lambda^n
\\ T^nxx^{-1}=x \lambda^nx^{-1}
\\ T^n=x \lambda^nx^{-1}
\\ T^{n+1}=T^nT=x \lambda^nx^{-1} x \lambda x^{-1}= x \lambda^{n+1} x^{-1}
\\T^{n+1}x=x \lambda^{n+1} x^{-1}x=x \lambda^{n+1}
$$

---

$$
P(x)=a_nx^n+ \dots +a_0
\\ P(T)=a_nT^n+ \dots +a_0
\\ \text{using part a from Exercise 1 if }\lambda^n \text{ is eigenvalue of }T^n \text{ then }a\lambda^n
\\ \text{ is eigenvalue of }aT^n
\\ \text{using part b from Exercise 1 if }T_1, T_2 
\\ \text{ are having same eigenvector then eigenvalue of their sum is equal to sum of each eigenvalue}
\\ P(T)x=(a_nT^n+ \dots +a_0)x=(a_nT^nx+ \dots +a_0x)
\\ \text{For each }a_nT^nx=a_n\lambda^nx
\\ \text{Using the 1-(b) eigenvalue of }P(T)=a_n\lambda^nx+\dots a_0
\\
\\a_n\lambda^n+ \dots +a_0 = P(\lambda)
\\
\\ \text{Therefore }x \text{ is an eigenvector of }P(T)\text{ belonging to }P(\lambda)
$$

(8) 4.4 Pr 3
$$
\text{Assume rotating on counterclock wise}
\\
\\ \text{Consider the plane as a real linear space,}  V = V_2(R) \text{ and let } T \text{ be a rotation of V through an angle of } 
\\ \frac{\pi}{2} \text{ radians. Although } T\text{	 has no eigenvectors, } 
\\ \text{ prove that every nonzero vector is an
eigenvector for }T^2
\\

\\ \text{let }T:V_2\rightarrow V_2 \text{ is a linear transformation that rotates }(x,y) \text{ with degree of }\theta
\\ \text{basis is }(1,0) (0,1)
\\ T((1,0))=(cos\theta,sin\theta)=cos\theta(1,0)+sin\theta(0,1)
\\ T((0,1))=(-sin\theta,cos\theta)=-sin\theta(1,0)+cos\theta(0,1)
\\
\\ \text{Therefore rotation matrix }T= \begin{bmatrix}cos\theta&-sin\theta \\ sin\theta &cos\theta \end{bmatrix}
\\ \text{Since }T \text{ is rotating with an angle of }\frac{\pi}{2} \text{ rad}
\\
\\T= \begin{bmatrix}cos\frac{\pi}{2}&-sin\frac{\pi}{2}\\ sin\frac{\pi}{2} &cos\frac{\pi}{2} \end{bmatrix}=\begin{bmatrix}0&-1\\ 1 &0 \end{bmatrix}
\\
\\ \vec x =(x,y)
\\ T(\vec x)=\begin{bmatrix}0&-1\\ 1 &0 \end{bmatrix}\begin{bmatrix}x\\y\end{bmatrix}=\begin{bmatrix}-y\\x\end{bmatrix}
$$

$$
\text{eigenvalue for T }
\\ \det(\lambda I \ - T)=0
\\ \det(\begin{bmatrix}\lambda&0\\ 0&\lambda \end{bmatrix}-\begin{bmatrix}0&-1\\ 1 &0 \end{bmatrix})
\\=\det(\begin{bmatrix}\lambda&1\\ -1&\lambda \end{bmatrix})
\\ = \lambda^2+1=0
\\ \text{satisfying eigenvalues are }-i,i \text{ that means there is no real eigenvalue for }T
\\
\\ T^2=\begin{bmatrix}0&-1\\ 1 &0 \end{bmatrix}\begin{bmatrix}0&-1\\ 1 &0 \end{bmatrix}
\\ = \begin{bmatrix}-1&0\\ 0 &-1 \end{bmatrix}
\\
\\ \text{eigenvalue is }
\det(\lambda I \ - T^2)=0
\\ \det(\begin{bmatrix}\lambda&0\\ 0&\lambda \end{bmatrix}-\begin{bmatrix}-1&0\\ 0 &-1 \end{bmatrix})
\\=\det(\begin{bmatrix}\lambda+1&0\\ 0&\lambda+1 \end{bmatrix})
\\ = (\lambda+1)^2=0
\\ \text{eigenvalue is }-1
\\
\\ T^2(\vec x)= \begin{bmatrix}-x\\-y\end{bmatrix}=(-1)\begin{bmatrix}x\\y\end{bmatrix}
\\ \text{Therefore every nonzero vector is an
eigenvector for }T^2
$$



