# Math 375

#### Geonho Roh

* 1.17 Pr 1
  $$
  \text{In each case, find an orthonormal basis for the subspace of }  V_3\text{ spanned by the given vectors}
  \\
  \\ \text{(a) } x_1 = (1, 1, 1), x_2 = (1,0,1), x_3 = (3,2,3) 
  \\ \text{(b) } x_1 = (1, 1, 1), x_2 = (-1,1,-1), x_3 = (1,0, 1)
  $$

$$
\text{(a) } x_1 = (1, 1, 1), x_2 = (1,0,1), x_3 = (3,2,3)
\\ \text{Since }2x_1 + x_2 =x_3 \text{ we can ignore }x_3
\\
\\ \text{Let }v_1 = x_1
\\ v_2 = x_2 - proj_{v_1}x_2= \begin{bmatrix}1 \\ 0\\1  \end{bmatrix}-\frac{<x_2,v_1>}{<v_1,v_1>}v_1
\\  =\begin{bmatrix}1 \\ 0\\1  \end{bmatrix}- \frac{2}{3}\begin{bmatrix}1 \\ 1\\1  \end{bmatrix}
=\begin{bmatrix}\frac{1}{3}  \\ -\frac{2}{3} \\\frac{1}{3}  \end{bmatrix}
$$

$$
\\ \text{Orthogonal basis is }\begin{bmatrix}1,\frac{1}{3} \\ 1,-\frac{2}{3}\\1,\frac{1}{3}  \end{bmatrix}
\\ \text{Change it to orthonormal}
\\ \begin{bmatrix}\frac{\sqrt{3}}{3},\frac{\sqrt{6}}{6} \\ \frac{\sqrt{3}}{3},-\frac{\sqrt{6}}{3}\\\frac{\sqrt{3}}{3},\frac{\sqrt{6}}{6}  \end{bmatrix}
$$

---------

$$
\text{(b) } x_1 = (1, 1, 1), x_2 = (-1,1,-1), x_3 = (1,0, 1)
\\ x_1-2x_3=x_2
\\ \text{Therefore we can ignore }x_2 \text{ and it is same as previous problem }(a)
\\ \text{Orthonormal basis for }(a) , (b)\text{ is same}
\\
\\\begin{bmatrix}\frac{\sqrt{3}}{3},\frac{\sqrt{6}}{6} \\ \frac{\sqrt{3}}{3},-\frac{\sqrt{6}}{3}\\\frac{\sqrt{3}}{3},\frac{\sqrt{6}}{6}  \end{bmatrix}
$$



* 1.17 Pr 2a 
  $$
  \text{n each case, find an orthonormal basis for the subspace of }  V_4\text{ spanned by the given vectors.}
  \\
  \\(a)\ x_1 = (1, 1,0, 0), x_2 = (0,1,1,0), x_3 = (0, 0, 1, 1), x_4 = (1,0,0, 1)
  $$

  $$
  \text{Since }x_1 + x_3 -x_2 = x_4 \text{ we can ignore }x_4
  \\ \text{Let }v_1 = x_1
  \\ v_2 = x_2 - proj_{v_1}x_2 =\begin{bmatrix}0\\1 \\ 1\\0  \end{bmatrix}-\frac{<x_2,v_1>}{<v_1,v_1>}v_1
  \\ = \begin{bmatrix}0\\1 \\ 1\\0  \end{bmatrix}-\frac{1}{2}\begin{bmatrix}1\\1 \\ 0\\0  \end{bmatrix}=\begin{bmatrix}-\frac{1}{2}\\\frac{1}{2} \\ 1\\0  \end{bmatrix}
  \\ v_3= x_3-\frac{<x_3,v_1>}{<v_1,v_1>}v_1-\frac{<x_3,v_2>}{<v_2,v_2>}v_2
  \\ = \begin{bmatrix}0\\0 \\ 1\\1  \end{bmatrix}-0(v_1)-\frac{1}{1.5}\begin{bmatrix}-\frac{1}{2}\\\frac{1}{2} \\ 1\\0  \end{bmatrix}
  $$

  $$
  = \begin{bmatrix}0\\0 \\ 1\\1  \end{bmatrix}-\frac{2}{3}\begin{bmatrix}-\frac{1}{2}\\\frac{1}{2} \\ 1\\0  \end{bmatrix}= \begin{bmatrix}\frac{1}{3}\\-\frac{1}{3}\\ \frac{1}{3}\\1  \end{bmatrix}
  \\
  \\ \text{Orthogonal basis is }\begin{bmatrix}1,-\frac{1}{2},\frac{1}{3}\\1,\frac{1}{2},-\frac{1}{3}\\ 0,1,\frac{1}{3}\\0,0,1  \end{bmatrix}
  \\ \text{Orthonormal basis is} \begin{bmatrix}\frac{\sqrt{2}}{2},-\frac{\sqrt{6}}{6},\frac{\sqrt{3}}{6}\\\frac{\sqrt{2}}{2},\frac{\sqrt{6}}{6},-\frac{\sqrt{3}}{6}\\ 0,\frac{\sqrt{6}}{3},\frac{\sqrt{3}}{6}\\0,0,\frac{\sqrt{3}}{2}  \end{bmatrix}
  $$

  

* 1.17 Pr 2b 
  $$
  (b)\ x_1= (1, 1,0, 1), x_2 = (1, 0,2, 1) x_3 = (1,2, -2, 1).
  \\
  $$

  $$
  v_1=x_1
  \\
  \\v_2=x_2 - proj_{v_1}x_2 =\begin{bmatrix}1\\1 \\ 0\\1  \end{bmatrix}-\frac{<x_2,v_1>}{<v_1,v_1>}v_1
  \\ = \begin{bmatrix}1\\0 \\ 2\\1  \end{bmatrix}- \frac{2}{3}\begin{bmatrix}1\\1 \\ 0\\1  \end{bmatrix}=\begin{bmatrix}\frac{1}{3}\\-\frac{2}{3}\\ 2\\\frac{1}{3}  \end{bmatrix}
  \\
  \\v_3= x_3-\frac{<x_3,v_1>}{<v_1,v_1>}v_1-\frac{<x_3,v_2>}{<v_2,v_2>}v_2
  \\ = \begin{bmatrix}1\\2 \\ -2\\1  \end{bmatrix}-\frac{4}{3}\begin{bmatrix}1\\1 \\ 0\\1  \end{bmatrix}+\begin{bmatrix}\frac{1}{3}\\-\frac{2}{3}\\ 2\\\frac{1}{3}  \end{bmatrix}=\begin{bmatrix}0\\0\\ 0\\0  \end{bmatrix} \text{ discard since its zero vector}
  $$

  $$
  \\
  \\ \text{Orthogonal basis is }\begin{bmatrix}1,\frac{1}{3}\\1 ,-\frac{2}{3}\\ 0,2\\1,\frac{1}{3}  \end{bmatrix}
  \\ \text{Orthonormal basis is }\begin{bmatrix}\frac{\sqrt{3}}{3},\frac{1}{\sqrt{42}}\\\frac{\sqrt{3}}{3} ,-\frac{2}{\sqrt{42}}\\ 0,\frac{6}{\sqrt{42}}\\\frac{\sqrt{3}}{3},\frac{1}{\sqrt{42}} \end{bmatrix}
  $$
  
  

* 1.17 Pr 3 
  $$
  \text{In the real linear space }C(0,\pi) \text{ with inner product }<x,y>=\int_{0}^{\pi}x(t)y(t)dt
  \\ \text{let }x(t)=cos(nt) \text{ for }n=0,1,2,3\dots
  \\ \text{Prove }y_0=\frac{1}{\sqrt{\pi}}\ \ \  y_n=\sqrt{\frac{2}{\pi}}cos(nt) \ n\geq1
  \\ \text{is forming orthonormal set and spanning same as }\{x_0,x_1\dots\}
  $$
   
  $$
  \text{To show they are orthonormal set}
  \\ \text{First prove they are orthogonal}
  \\
  \\ \text{There can be two cases for choosing elements in y: }y_0 \text{ and }y_n (n \geq 1), y_a \text{ and } y_b \ \ a,b \geq1
  \\ y_0=\frac{1}{\sqrt{\pi}}\ \ \  y_n=\sqrt{\frac{2}{\pi}}cos(nt) \ \  n\geq1
  \\ <y_0,y_n> = \int_{0}^{\pi}\frac{1}{\sqrt{\pi}}\sqrt{\frac{2}{\pi}}cos(nt)
  \\ = \int_{0}^{\pi}\frac{\sqrt{2}}{\pi}cos(nt)=\frac{\sqrt{2}}{\pi}\int_{0}^{\pi}cos(nt)=\frac{\sqrt{2}}{\pi}\Big|\frac{1}{n}sin(nt)\Big|_{0}^{\pi}=0
  $$
  
  $$
  y_a=\sqrt{\frac{2}{\pi}}cos(at) \text{ and }y_b=\sqrt{\frac{2}{\pi}}cos(bt)
  \\<y_a,y_b>=\int_{0}^{\pi}\sqrt{\frac{2}{\pi}}cos(at)\sqrt{\frac{2}{\pi}}cos(bt)
  \\=\frac{2}{\pi}\int_{0}^{\pi}cos(at)cos(bt)=\frac{2}{\pi}\int_{0}^{\pi}\frac{1}{2}[cos(at+bt)cos(at-bt)]
  \\=\frac{2}{\pi}\frac{1}{2}\int_{0}^{\pi}[cos(at+bt)+cos(at-bt)] 
  \\\frac{2}{\pi}\frac{1}{2}\int_{0}^{\pi}[cos((a+b)t)+cos((a-b)t)] =\frac{1}{\pi}\int_{0}^{\pi}cos((a+b)t)+\frac{1}{\pi}\int_{0}^{\pi}cos((a-b)t)
  \\=\frac{1}{\pi}\Big|\frac{1}{a+b}sin((a+b)t)+\frac{1}{a-b}sin((a-b)t)\Big|_{0}^{\pi}=0
  $$
  
  $$
  \text{In every cases inner product is 0 therefore it is orthogonal}
  \\ \text{Next, show the set is orthonormal}
  \\ \text{When }y_0
  \\<y_0,y_0>=\int_{0}^{\pi}\frac{1}{\sqrt{\pi}}\frac{1}{\sqrt{\pi}}=\int_{0}^{\pi}\frac{1}{\pi}
  \\ = \Big|\frac{1}{\pi}t\Big|_{0}^{\pi}=1
  \\ \text{therefore }y_0 \text{ is normalized}
  \\
  \\ \text{when }y_n , n\geq1
  \\ <y_n,y_n>=\int_{0}^{\pi}\sqrt{\frac{2}{\pi}}cos(nt)\sqrt{\frac{2}{\pi}}cos(nt)=\frac{2}{\pi}\int_{0}^{\pi}cos^2(nt)
  \\=\frac{2}{\pi}\int_{0}^{\pi}\frac{1+cos(2nt)}{2} =\frac{2}{\pi}\int_{0}^{\pi}\frac{1}{2}+\frac{2}{\pi}\int_{0}^{\pi}\frac{cos(2nt)}{2}
  \\= \frac{2}{\pi}\Big|\frac{1}{2}t\Big|_{0}^{\pi}+\frac{2}{\pi}\Big|\frac{sin(2nt)}{4n}\Big|_{0}^{\pi}
  \\= \frac{2}{\pi}\frac{\pi}{2}=1
  \\ \text{therfore }y_n \text{ is normalized}
  \\
  \\ \text{The set is orthonormal}
  $$

$$
\text{And to it is enough to show }\{y_0,y_1\dots\} \text{can be obtained by scalar multiplication of }
\\ \{x_0,x_1\dots\} 
\\ \text{Since } \ x(t)=cos(nt) \text{ for }n=0,1,2,3\dots
\\ y_0=\frac{1}{\sqrt{\pi}}\ \ \  y_n=\sqrt{\frac{2}{\pi}}cos(nt) \ n\geq 1
\\
\\ \text{There are }c_k \in \R \text{ which satisfy }c_kx_k = y_k
\\ \text{ So they are spanning same space}
$$



* 1.17 Pr 6 
  $$
  \text{In the real number space }C(1,3) \text{ with inner product }<f.g>=\int_{1}^{3}f(x)g(x)dx
  \\ \text{let }f(x) = \frac{1}{x} \text{ and show that the constant polynomial }g \text{ nearest to }f \text{ is }g=\frac{1}{2}log(3) 
  \\ \text{ Compute } \|g-f\|^2 \text{ for this g}
  $$

  $$
  {1} \text{ is a basis for }g
  \\ \frac{\sqrt{2}}{2}\text{is orthonormal basis}
  $$

  $$
  \text{let }w=\{\frac{\sqrt{2}}{2}\}
  \\ proj_{w}f(x)=proj_{w}\frac{1}{x}
  \\ = \frac{<f,w>}{<w,w>}w=\frac{\frac{\sqrt2 ln(3)}{2}}{1}\frac{\sqrt{2}}{2}
  \\=\frac{ln(3)}{2}
  \\ 
  \\ \text{Therefore the constant polynomial g nearest to f is }\frac{ln(3)}{2}
  $$

  $$
  \\
  \\ \text{Compute }\|g-f\|^2 , g=\frac{ln(3)}{2}
  \\ g-f = \frac{ln(3)}{2} - \frac{1}{x}= \frac{ln(3)x-2}{2x}
  \\ \|g-f\|^2 =<g-f,g-f>=\int_{1}^{3}\frac{ln(3)x-2}{2x}\frac{ln(3)x-2}{2x}dx
  \\=\int_{1}^{3}\frac{ln^2(3)x^2-4ln(3)x+4}{4x^2}dx=\int_{1}^{3}\frac{ln^2(3)x^2}{4x^2}dx+\int_{1}^{3}\frac{-4ln(3)x}{4x^2}dx+\int_{1}^{3}\frac{4}{4x^2}dx
  \\=\frac{ln^2(3)}{2}+(-1)ln^2(3)+ \frac{2}{3}=-\frac{ln^2(3)}{2}+ \frac{2}{3}
  $$

  

* 1.17 Pr 9
  $$
  \text{In the real number space }C(0,2\pi) \text{ with inner product }<f.g>=\int_{0}^{2\pi}f(x)g(x)dx
  \\ \text{let }f(x) = x \text{ In the subspace spanned by } u_0(x)=1, u_1(x)=cos(x), u_2(x)=sin(x), 
  \\ \text{Find  the trigometric polynomial nearest to }f
  $$

  $$
  \text{Get projection of }f(x)\text{ onto }u_0,u_1,u_2
  \\
  \\ proj_{u_0}f(x)=\frac{<f,u_0>}{<u_0,u_0>}u_0=\frac{2\pi^2}{2\pi}=\pi
  \\
  \\ proj_{u_1}f(x)=\frac{<f,u_1>}{<u_1,u_1>}u_1=\frac{\int_{0}^{2\pi}xcos(x)dx}{\int_{0}^{2\pi}1+cos(2x)dx}cos(x)
  \\=\frac{\Big|xsin(x) \Big|_{0}^{2\pi}-\int_{0}^{2\pi}sin(x)dx}{\frac{1}{2}\int_{0}^{2\pi}1+cos(2x)dx}cos(x)
  \\=\frac{-\Big|-cos(x)\Big|_{0}^{2\pi}}{\frac{1}{2}\int_{0}^{2\pi}1+cos(2x)dx}cos(x), \ \text{ Since }-\Big|-cos(x)\Big|_{0}^{2\pi}=0
  \\ \frac{-\Big|-cos(x)\Big|_{0}^{2\pi}}{\frac{1}{2}\int_{0}^{2\pi}1+cos(2x)dx}cos(x)=0
  $$

  $$
  proj_{u_2}f(x)=\frac{<f,u_2>}{<u_2,u_2>}u_2=\frac{\int_{0}^{2\pi}xsin(x)dx}{\int_{0}^{2\pi}1-cos(2x)dx}sin(x)
  \\ =\frac{\Big|-xcos(x) \Big|_{0}^{2\pi}+\int_{0}^{2\pi}cos(x)dx}{\frac{1}{2}\int_{0}^{2\pi}1+cos(2x)dx}sin(x)
  \\ =\frac{-2\pi+0}{\frac{1}{2}\Big|x+\frac{1}{2}sin(2x)\Big|_{0}^{2\pi}}sin(x)
  \\ =-2sin(x)
  $$

  $$
  \\
  \\ \text{Therefore }g(x) = \pi-2sin(x)
  $$

  

